

Practice Problems Set 13

Fall 25

1. Floyd-Hoare Verification

The following program purports to compute the factorial of a nonnegative integer n . Prove the program's partial correctness (i.e. that if it halts, it computes the factorial of n , for any nonnegative input n), by giving a Floyd-style proof. Do this by giving an inductive invariant at every point in the program.

```
int r, t;  
r = 1;  
t = n;  
while (t > 0) {  
    r = r * t;  
    t = t - 1;  
}  
return r;
```

Solution:

We first construct a Hoare triple for the whole program by annotating the pre- and post-conditions, namely $n \geq 0$ and $r = n!$. Then we annotate the program with inductive invariant at every point in the program to form a Floyd-style proof:

```
{Pre :  $n \geq 0$ }  
int r, t;  
r = 1;  
{ $n \geq 0 \wedge r = 1$ }  
t = n;  
{ $n \geq 0 \wedge n! = r \times t! \wedge 0 \leq t \leq n$ }  
while (t > 0) {  
    r = r * t;  
    { $n \geq 0 \wedge n! = r \times (t - 1)! \wedge 0 < t \leq n$ }  
    t = t - 1;  
}  
return r;  
{Post :  $r = n!$ }
```

2. Termination

Consider the following program:

```

int a,b;
a = 1000; b = 0;
while (a != 0 || b != 0) {
    if (b == 0) {
        a = a-1;
        b = f();
    }
    else
        b = b-1;
}

```

In the above, $f()$ is a function that returns arbitrary positive numbers each time it is called (it need not return the same number on two successive invocations). Think of $f()$ as, say, a function that returns a number from the environment (input). More formally, all that we know is that $f()$ returns a value greater than 0.

Prove that the above code terminates always by giving a proof based on ranking functions.

Solution:

We use the ranking function $V(a, b) = \langle a, b \rangle$ with lexicographical order. The annotated program below shows the rank decreases in both branches:

```

while (a != 0 || b != 0) {
    decreases  $\langle a, b \rangle$ 
    // Capture rank at loop entry:  $V_{old} = \langle a, b \rangle$ 
    if (b == 0) {
        a = a-1;
        b = f();
        // New state:  $\langle a-1, f() \rangle$ 
        // Decrease:  $\langle a-1, f() \rangle \prec_{lex} \langle a, 0 \rangle$ 
        // (Decreases because first component  $a$  became smaller)
    }
    else {
        b = b-1;
        // New state:  $\langle a, b-1 \rangle$ 
        // Decrease:  $\langle a, b-1 \rangle \prec_{lex} \langle a, b \rangle$ 
        // (Decreases because first component equal, second smaller)
    }
}

```